finish clarification when a program fails
now bir_program_terminationTheory is extended to reason about when
status code BST_Failed is produced. Unluckily there was a cyclic
dependency with required moving some theorems form
bir_program_varsScript.sml to bir_program_blocksScript.sml

src/core-props/bir_program_terminationScript.sml
@@ -1,7 +1,11 @@
 open HolKernel Parse boolLib bossLib;
 open bir_programTheory bir_program_valid_stateTheory HolBACoreSimps;
 open bir_program_multistep_propsTheory bir_auxiliaryTheory
+open bir_typing_expTheory bir_envTheory
+open bir_typing_progTheory
 open bir_valuesTheory bir_immTheory
+open bir_program_env_orderTheory
+open pred_setTheory
 
 val _ = new_theory "bir_program_termination";
 
@@ -427,7 +431,6 @@ METIS_TAC[bir_exec_stmt_status_assumption]);
 (* Status AssertionViolated *)
 (*****************************)
 
-
 val bir_exec_stmtB_status_assertion = store_thm ("bir_exec_stmtB_status_assertion",
 ``!st stmt. (st.bst_status <> BST_AssertionViolated) ==>
             ((bir_exec_stmtB_state stmt st).bst_status = BST_AssertionViolated) ==>
@@ -485,6 +488,363 @@ CASE_TAC >> (
   ASM_SIMP_TAC (std_ss++holBACore_ss) [bir_state_set_failed_def, GSYM bir_exec_stmt_state_def]
 ) >>
 METIS_TAC[bir_exec_stmt_status_assertion]);
+
+
+
+
+(*****************)
+(* Status Failed *)
+(*****************)
+
+(* For failing there are many possible reasons:
+
+   - an invalid PC
+   - the variable name of a newly declared var is already present in the environment
+   - an not-well-typed statement, i.e. an expression returns a different type than expected
+   - evaluation of expression fails
+   - assigning to a undeclared var or one of wrong type
+   - ...
+
+  This is shown formally below. Since the possible conditions are varied,
+  it is shown separately for each statement. *)
+
+val bir_exec_stmtB_status_failed_Declare = store_thm ("bir_exec_stmtB_status_failed_Declare",
+``!st stmt v. (st.bst_status <> BST_Failed) ==>
+            (((bir_exec_stmtB_state (BStmt_Declare v) st).bst_status = BST_Failed) <=>
+             (bir_env_varname_is_bound st.bst_environ (bir_var_name v)))``,
+
+REPEAT GEN_TAC >>
+Cases_on `st.bst_environ` >> rename1 `BEnv env` >>
+ASM_SIMP_TAC std_ss [bir_exec_stmtB_state_def, bir_exec_stmtB_def,
+  bir_exec_stmt_declare_def, bir_env_update_def, bir_state_set_failed_def] >>
+REPEAT CASE_TAC >> FULL_SIMP_TAC (std_ss++holBACore_ss) [] >>
+rename1 `bir_var_type vv` >>
+Cases_on `bir_var_type vv` >> (
+  FULL_SIMP_TAC std_ss [bir_declare_initial_value_def] >>
+  BasicProvers.VAR_EQ_TAC >>
+  FULL_SIMP_TAC std_ss [type_of_bir_val_def]
+));
+
+
+val bir_exec_stmtB_status_failed_Assign = store_thm ("bir_exec_stmtB_status_failed_Assign",
+``!st stmt v e. (st.bst_status <> BST_Failed) ==>
+                (((bir_exec_stmtB_state (BStmt_Assign v e) st).bst_status = BST_Failed) <=>
+                 (~(bir_env_var_is_declared st.bst_environ v) \/
+                  (type_of_bir_val (bir_eval_exp e st.bst_environ) <> SOME (bir_var_type v))))``,
+
+REPEAT GEN_TAC >>
+Cases_on `st.bst_environ` >> rename1 `BEnv env` >>
+ASM_SIMP_TAC std_ss [bir_exec_stmtB_state_def, bir_exec_stmtB_def,
+  bir_exec_stmt_assign_def, bir_env_update_def, bir_state_set_failed_def,
+  LET_DEF, bir_env_write_def, bir_env_var_is_declared_ALT_DEF] >>
+REPEAT CASE_TAC >> FULL_SIMP_TAC (std_ss++holBACore_ss) []);
+
+
+val bir_exec_stmtB_status_failed_cond_exp_aux = prove (
+ ``!v. (type_of_bir_val v = SOME BType_Bool) <=>
+       (case bir_dest_bool_val v of
+         | NONE => F
+         | SOME _ => T)``,
+
+REPEAT GEN_TAC >>
+SIMP_TAC std_ss [GSYM bir_val_checker_TO_type_of,
+  optionTheory.option_case_compute] >>
+METIS_TAC[bir_dest_bool_val_EQ_NONE, optionTheory.option_CLAUSES]);
+
+
+val bir_exec_stmtB_status_failed_Assert = store_thm ("bir_exec_stmtB_status_failed_Assert",
+``!st stmt e. (st.bst_status <> BST_Failed) ==>
+              (((bir_exec_stmtB_state (BStmt_Assert e) st).bst_status = BST_Failed) <=>
+              (type_of_bir_val (bir_eval_exp e st.bst_environ) <> SOME BType_Bool))``,
+
+REPEAT GEN_TAC >>
+SIMP_TAC std_ss [bir_exec_stmtB_state_def, bir_exec_stmtB_def,
+  bir_exec_stmt_assert_def, bir_exec_stmtB_status_failed_cond_exp_aux] >>
+Cases_on `bir_dest_bool_val (bir_eval_exp e st.bst_environ)` >> (
+  SIMP_TAC (std_ss++bir_TYPES_ss++boolSimps.LIFT_COND_ss) [bir_state_set_failed_def]
+));
+
+
+val bir_exec_stmtB_status_failed_Assume = store_thm ("bir_exec_stmtB_status_failed_Assume",
+``!st stmt e. (st.bst_status <> BST_Failed) ==>
+              (((bir_exec_stmtB_state (BStmt_Assume e) st).bst_status = BST_Failed) <=>
+              (type_of_bir_val (bir_eval_exp e st.bst_environ) <> SOME BType_Bool))``,
+
+REPEAT GEN_TAC >>
+SIMP_TAC std_ss [bir_exec_stmtB_state_def, bir_exec_stmtB_def,
+  bir_exec_stmt_assume_def, bir_exec_stmtB_status_failed_cond_exp_aux] >>
+Cases_on `bir_dest_bool_val (bir_eval_exp e st.bst_environ)` >> (
+  SIMP_TAC (std_ss++bir_TYPES_ss++boolSimps.LIFT_COND_ss) [bir_state_set_failed_def]
+));
+
+
+val bir_exec_stmtB_status_failed_Observe = store_thm ("bir_exec_stmtB_status_failed_Observe",
+``!st stmt e. (st.bst_status <> BST_Failed) ==>
+              (((bir_exec_stmtB_state (BStmt_Observe ec es osf) st).bst_status = BST_Failed) <=>
+              (type_of_bir_val (bir_eval_exp ec st.bst_environ) <> SOME BType_Bool))``,
+
+REPEAT GEN_TAC >>
+SIMP_TAC std_ss [bir_exec_stmtB_state_def, bir_exec_stmtB_def,
+  bir_exec_stmt_observe_def] >>
+Cases_on `bir_dest_bool_val (bir_eval_exp ec st.bst_environ)` >| [
+  FULL_SIMP_TAC (std_ss++holBACore_ss) [bir_state_set_failed_def,
+    bir_dest_bool_val_EQ_NONE, bir_val_checker_TO_type_of],
+
+  FULL_SIMP_TAC (std_ss++boolSimps.LIFT_COND_ss++holBACore_ss) [
+    bir_dest_bool_val_EQ_SOME, BType_Bool_def]
+]);
+
+
+val bir_exec_stmtE_status_failed_jmp_to_label = store_thm ("bir_exec_stmtE_status_failed_jmp_to_label",
+``!st stmt p l. (st.bst_status <> BST_Failed) ==>
+                ((bir_exec_stmt_jmp_to_label p l st).bst_status <> BST_Failed)``,
+SIMP_TAC (std_ss++boolSimps.LIFT_COND_ss++bir_TYPES_ss) [bir_exec_stmt_jmp_to_label_def]);
+
+
+val bir_eval_label_exp_EQ_NONE = store_thm ("bir_eval_label_exp_EQ_NONE",
+``!le env. (bir_eval_label_exp le env = NONE) <=>
+           (?e. (le = BLE_Exp e) /\
+                ~(bir_val_is_Imm (bir_eval_exp e env)))``,
+
+Cases >> (
+  SIMP_TAC (std_ss++bir_TYPES_ss) [bir_eval_label_exp_def,
+    bir_val_is_Imm_def]
+) >>
+REPEAT GEN_TAC >> CASE_TAC);
+
+
+val bir_exec_stmtE_status_failed_Jmp = store_thm ("bir_exec_stmtE_status_failed_Jmp",
+``!st stmt p le. (st.bst_status <> BST_Failed) ==>
+                 (((bir_exec_stmtE p (BStmt_Jmp le) st).bst_status = BST_Failed) <=>
+                 (bir_eval_label_exp le st.bst_environ = NONE))``,
+
+REPEAT GEN_TAC >>
+SIMP_TAC std_ss [bir_exec_stmtE_def, bir_exec_stmt_jmp_def] >>
+CASE_TAC >> (
+  SIMP_TAC (std_ss++bir_TYPES_ss) [bir_exec_stmtE_status_failed_jmp_to_label,
+    bir_state_set_failed_def]
+));
+
+
+val bir_exec_stmtE_status_failed_CJmp = store_thm ("bir_exec_stmtE_status_failed_CJmp",
+``!st stmt p ce le1 le2.
+     (st.bst_status <> BST_Failed) ==>
+     (((bir_exec_stmtE p (BStmt_CJmp ce le1 le2) st).bst_status = BST_Failed) <=>
+      case bir_dest_bool_val (bir_eval_exp ce st.bst_environ) of
+         NONE => T
+       | SOME T => (bir_eval_label_exp le1 st.bst_environ = NONE)
+       | SOME F => (bir_eval_label_exp le2 st.bst_environ = NONE))``,
+
+REPEAT GEN_TAC >>
+SIMP_TAC std_ss [bir_exec_stmtE_def, bir_exec_stmt_cjmp_def,
+  bir_exec_stmt_jmp_def] >>
+REPEAT CASE_TAC >> (
+  SIMP_TAC (std_ss++bir_TYPES_ss++boolSimps.LIFT_COND_ss) [
+    bir_exec_stmtE_status_failed_jmp_to_label,
+    bir_state_set_failed_def]
+));
+
+
+
+val bir_exec_stmtE_status_failed_Halt = store_thm ("bir_exec_stmtE_status_failed_Halt",
+``!st stmt p e.
+     (((bir_exec_stmtE p (BStmt_Halt e) st).bst_status <> BST_Failed))``,
+
+SIMP_TAC (std_ss++bir_TYPES_ss) [bir_exec_stmtE_def, bir_exec_stmt_halt_def]);
+
+
+
+
+(***********************************************)
+(* Well-formed progs with all vars initialised *)
+(***********************************************)
+
+(* As shown above: the reasons for a statement to produce status
+   BST_Failed are varied. If we assume however, that all initialisations
+   have been done already, we have a simple overapproximation.
+
+   If a program
+
+   - is well-formed
+   - does not contain assign
+   - is run in from a state
+       + with a valid PC
+       + all vars used by the program initialised
+       + status not failed
+
+  then this execution will not fail.
+*)
+
+
+val bir_eval_label_exp_NEQ_NONE_WF_INITIALISED = store_thm ("bir_eval_label_exp_NEQ_NONE_WF_INITIALISED",
+``!le env.
+  bir_is_well_typed_label_exp le ==>
+  bir_env_vars_are_initialised env (bir_vars_of_label_exp le) ==>
+  bir_eval_label_exp le env <> NONE``,
+
+Cases >- SIMP_TAC std_ss [bir_eval_label_exp_def] >>
+SIMP_TAC std_ss [bir_eval_label_exp_def,
+  bir_is_well_typed_label_exp_def, bir_vars_of_label_exp_def] >>
+REPEAT STRIP_TAC >>
+rename1 `type_of_bir_exp e` >>
+Cases_on `type_of_bir_exp e` >> FULL_SIMP_TAC std_ss [bir_type_is_Imm_def] >>
+BasicProvers.VAR_EQ_TAC >>
+rename1 `_ = SOME (BType_Imm s)` >>
+`type_of_bir_val (bir_eval_exp e env) = SOME (BType_Imm s)` by
+  METIS_TAC[type_of_bir_exp_THM_with_init_vars] >>
+FULL_SIMP_TAC std_ss [type_of_bir_val_EQ_ELIMS] >>
+FULL_SIMP_TAC (std_ss++bir_TYPES_ss) []);
+
+
+val bir_exec_stmt_NOT_FAIL_AFTER_INIT = store_thm ("bir_exec_stmt_NOT_FAIL_AFTER_INIT",
+``!st p stmt.
+
+    (st.bst_status <> BST_Failed) ==>
+    (bir_is_well_typed_stmt stmt) ==>
+    (bir_env_vars_are_initialised st.bst_environ (bir_vars_of_stmt stmt) ) ==>
+
+    (((bir_exec_stmt_state p stmt st).bst_status = BST_Failed) <=>
+     (?v. stmt = BStmtB (BStmt_Declare v)))``,
+
+REPEAT STRIP_TAC >>
+Cases_on `stmt` >- (
+  rename1 `BStmtB stmt` >>
+  FULL_SIMP_TAC (std_ss++bir_TYPES_ss++boolSimps.LIFT_COND_ss++pairSimps.gen_beta_ss) [
+    bir_exec_stmt_state_def, bir_exec_stmt_def,
+    LET_DEF, GSYM bir_exec_stmtB_state_def, bir_vars_of_stmt_def, bir_is_well_typed_stmt_def] >>
+
+  Cases_on `stmt` >> (
+    FULL_SIMP_TAC (list_ss++holBACore_ss) [
+      bir_exec_stmtB_status_failed_Declare,
+      bir_exec_stmtB_status_failed_Assign,
+      bir_exec_stmtB_status_failed_Assert,
+      bir_exec_stmtB_status_failed_Assume,
+      bir_exec_stmtB_status_failed_Observe,
+
+      type_of_bir_exp_THM_with_init_vars,
+      bir_vars_of_stmtB_def, bir_is_well_typed_stmtB_def,
+      bir_env_vars_are_initialised_INSERT, bir_env_vars_are_initialised_EMPTY,
+      bir_env_vars_are_initialised_UNION, IMAGE_INSERT, BIGUNION_INSERT,
+      bir_env_var_is_declared_weaken, bir_env_var_is_initialised_weaken]
+  )
+) >>
+
+rename1 `BStmtE stmt` >>
+FULL_SIMP_TAC (std_ss++bir_TYPES_ss++boolSimps.LIFT_COND_ss) [
+  bir_exec_stmt_state_def, bir_exec_stmt_def,
+  bir_vars_of_stmt_def, bir_is_well_typed_stmt_def] >>
+Cases_on `stmt` >> (
+  FULL_SIMP_TAC (std_ss++holBACore_ss) [
+     bir_is_well_typed_stmtE_def,
+     bir_vars_of_stmtE_def,
+     bir_env_vars_are_initialised_UNION,
+     bir_exec_stmtE_status_failed_Jmp,
+     bir_exec_stmtE_status_failed_CJmp,
+     bir_exec_stmtE_status_failed_Halt,
+     bir_eval_label_exp_NEQ_NONE_WF_INITIALISED]
+) >>
+(* CJmp *)
+CASE_TAC >>
+FULL_SIMP_TAC std_ss [bir_dest_bool_val_EQ_NONE,
+  bir_val_checker_TO_type_of] >>
+METIS_TAC[type_of_bir_exp_THM_with_init_vars]);
+
+
+
+val bir_program_contains_declarations_def = Define
+`bir_program_contains_declarations p <=>
+  (?v. (BStmtB (BStmt_Declare v)) IN bir_stmts_of_prog p)`
+
+val bir_program_contains_declarations_EVAL = store_thm ("bir_program_contains_declarations_EVAL",
+``!p.
+  bir_program_contains_declarations (BirProgram p) <=>
+  EXISTS (\bl. EXISTS (\stmt. case stmt of
+      BStmt_Declare _ => T
+    | _ => F) bl.bb_statements) p``,
+
+SIMP_TAC (list_ss++bir_TYPES_ss) [bir_program_contains_declarations_def,
+  bir_stmts_of_prog_def, bir_stmts_of_block_def,
+  IN_BIGUNION, IN_IMAGE, PULL_EXISTS, listTheory.EXISTS_MEM] >>
+REPEAT STRIP_TAC >> EQ_TAC >> REPEAT STRIP_TAC >| [
+  rename1 `BStmt_Declare v` >>
+  rename1 `MEM bl p` >>
+  Q.EXISTS_TAC `bl` >>
+  Q.EXISTS_TAC `BStmt_Declare v` >>
+  ASM_SIMP_TAC (std_ss++bir_TYPES_ss) [],
+
+  Cases_on `stmt` >> FULL_SIMP_TAC (std_ss++bir_TYPES_ss) [] >>
+  METIS_TAC[]
+]);
+
+
+
+val bir_exec_step_NOT_FAIL_AFTER_INIT = store_thm ("bir_exec_step_NOT_FAIL_AFTER_INIT",
+``!st p.
+    (bir_is_well_typed_program p) ==>
+    ~(bir_program_contains_declarations p) ==>
+    (st.bst_status <> BST_Failed) ==>
+    (bir_env_vars_are_initialised st.bst_environ (bir_vars_of_program p)) ==>
+    (bir_is_valid_pc p st.bst_pc) ==>
+
+    ((bir_exec_step_state p st).bst_status <> BST_Failed)``,
+
+REPEAT STRIP_TAC >>
+POP_ASSUM MP_TAC >>
+MP_TAC (Q.SPECL [`p`, `st`] bir_exec_step_state_valid_THM) >>
+Cases_on `bir_state_is_terminated st` >> ASM_SIMP_TAC std_ss [] >>
+STRIP_TAC >>
+MP_TAC (Q.SPECL [`st`, `p`, `stmt`] bir_exec_stmt_NOT_FAIL_AFTER_INIT) >>
+ASM_SIMP_TAC std_ss [] >>
+
+`stmt IN bir_stmts_of_prog p` by METIS_TAC[bir_get_current_statement_stmts_of_prog] >>
+` bir_vars_of_stmt stmt SUBSET bir_vars_of_program p` by
+   METIS_TAC[bir_get_current_statement_vars_of] >>
+`bir_env_vars_are_initialised st.bst_environ (bir_vars_of_stmt stmt)` by
+   METIS_TAC[bir_env_vars_are_initialised_SUBSET] >>
+FULL_SIMP_TAC std_ss [bir_is_well_typed_program_ALT_DEF,
+  bir_program_contains_declarations_def] >>
+METIS_TAC[]);
+
+
+val bir_exec_infinite_steps_fun_NOT_FAIL_AFTER_INIT = store_thm ("bir_exec_infinite_steps_fun_NOT_FAIL_AFTER_INIT",
+``!p i st.
+    (bir_is_well_typed_program p) ==>
+    ~(bir_program_contains_declarations p) ==>
+    (st.bst_status <> BST_Failed) ==>
+    (bir_env_vars_are_initialised st.bst_environ (bir_vars_of_program p)) ==>
+    (bir_is_valid_pc p st.bst_pc) ==>
+
+    ((bir_exec_infinite_steps_fun p st i).bst_status <> BST_Failed)``,
+
+
+GEN_TAC >> Induct >> (
+  SIMP_TAC std_ss [bir_exec_infinite_steps_fun_REWRS]
+) >>
+REPEAT STRIP_TAC >>
+Q.PAT_X_ASSUM `!st. _` (MP_TAC o Q.SPEC `bir_exec_step_state p st`) >>
+ASM_SIMP_TAC std_ss [bir_exec_step_NOT_FAIL_AFTER_INIT,
+  bir_exec_step_valid_pc] >>
+
+MATCH_MP_TAC (SIMP_RULE std_ss [AND_IMP_INTRO] bir_env_vars_are_initialised_ORDER) >>
+Q.EXISTS_TAC `st.bst_environ` >>
+ASM_SIMP_TAC std_ss [bir_exec_step_ENV_ORDER]);
+
+
+val bir_exec_step_n_fun_NOT_FAIL_AFTER_INIT = store_thm ("bir_exec_step_n_fun_NOT_FAIL_AFTER_INIT",
+``!p i st.
+    (bir_is_well_typed_program p) ==>
+    ~(bir_program_contains_declarations p) ==>
+    (st.bst_status <> BST_Failed) ==>
+    (bir_env_vars_are_initialised st.bst_environ (bir_vars_of_program p)) ==>
+    (bir_is_valid_pc p st.bst_pc) ==>
+
+    ((let (l, n, st') = bir_exec_step_n p st i in st').bst_status <> BST_Failed)``,
+
+REPEAT STRIP_TAC >>
+`?l n st'. bir_exec_step_n p st i = (l, n, st')` by METIS_TAC[pairTheory.PAIR] >>
+FULL_SIMP_TAC std_ss [LET_DEF] >>
+FULL_SIMP_TAC std_ss [bir_exec_step_n_EQ_THM] >>
+METIS_TAC[bir_exec_infinite_steps_fun_NOT_FAIL_AFTER_INIT]);
 
 
 val _ = export_theory();
